1. Oblicz pochodne funkcji

    1) $y = \frac{1}{3}x^3 - \frac{3}{2}x^4 + \frac{13}{5}x^5 - 2x^6$
    2) $y = 5x^{15} - x^2 + \frac{1}{3}x - 2$
    3) $y = ax^3 + \frac{b}{x} + c$
    4) $y = \frac{4}{x^3}$
    5) $y = 9x^7 + 3x^{-5} - 3x^{-11}$
    6) $y = 3x^{7/3} - 4x^{13/4} + \frac{4}{7}x^{-1/2} + 7^{3/2}$
    7) $y = \sqrt[3]{x^2}$
    8) $y = 5\sqrt[3]{x^7}$
    9) $y = 3\sqrt[3]{x} - x^3 + \frac{2}{3}\sqrt[3]{x^4}$
    10) $y = \sqrt{x} - 5\sqrt[3]{x^2} - 2\sqrt{x^3}$
    11) $y = \frac{2}{\sqrt{x}} - \frac{3}{\sqrt{x^3}}$
    12) $y = \frac{5}{7\sqrt[3]{x}} - 2x^7 + \frac{3}{2\sqrt{x}}$
    13) $x = t^3\sqrt{t}$
    14) $y = \frac{2}{x^3\sqrt{x}}$
    15) $y = (2\sqrt[3]{x^2}-x)(4\sqrt[3]{x^4}+2\sqrt[3]{x^5}+x^2)$
    16) $y = (4x^2-2x\sqrt{x}+x)(2x+\sqrt{x})$
    17) $y = \frac{3}{3x-2}$
    18) $y = \frac{5}{2x^2-5x+1}$
    19) $y = \frac{3x^2}{7x^5-x+2}$
    20) $y = \frac{8x^3}{x^3+x-1}$
    21) $y = \frac{x+1}{x-1}$
    22) $y = \frac{5x^2+x-2}{x^2+7}$
    23) $y = \frac{x^2-2x+3}{x^2+2x-3}$
    24) $y = \frac{3}{(1-x^2)(1-2x^3)}$
    25) $y = \frac{\sqrt[3]{x}}{1-\sqrt[3]{x}}$
    26) $z = \frac{1+\sqrt{t}}{1+\sqrt{2t}}$
    27) $s = (3t+1)^7$
    28) $v = (4z^2-5z+13)^5$
    29) $x = (\frac{1}{t}+4)^4$
    30) $s = (\frac{7t^2-\frac{t}{2}+6}{t})^6$
    31) $y = \sqrt{x^2-4}$
    32) $z = \sqrt{ax^2+bx+c}$
    33) $y = \frac{1}{\sqrt{2-3t}}$
    34) $s = \frac{1}{\sqrt{6t-t^2}}$
    35) $y = \frac{1}{\sqrt[3]{(2-x^3)^4}}$
    36) $y = \frac{a}{\sqrt[p]{(a+bx)^r}}$
    37) $y = \frac{1}{(b-x^n)^m}$
    38) $y = \sqrt[4]{(x-1)^3}$
    39) $u = \frac{1}{v-\sqrt{a^2+b^2}}$
    40) $y = \sqrt{\frac{a-x}{a^2-x^2}}$, $a>0$
    41) $v = \frac{z}{\sqrt{a^2-z^2}}$
    42) $y = \frac{3\sqrt{x}}{x^2+1}$
    43) $y = \frac{x^2}{\sqrt[3]{x^3+1}}$
    44) $z = \sqrt{\frac{x^2-3x+2}{x^2-7x+12}}$
    45) $z = \sqrt{\frac{a^2-x^2}{a^2+x^2}}$
    46) $s = \sqrt{\frac{1-\sqrt{t}}{1+\sqrt{t}}}$
    47) $u = \frac{\sqrt{1+v}-\sqrt{1-v}}{\sqrt{1+v}+\sqrt{1-v}}$
    48) $y=u(x)v(x)w(x)$
    49) $v = \cos \frac{t}{a}$, $a \ne 0$
    50) $x = a \sin bt$
    51) $y = a \sin \frac{a}{x}$
    52) $z = 2x+\sin 2x$
    53) $s = \sin^2 3t$
    54) $v = 4\cos^5 \frac{t}{4}$
    55) $s = \frac{1}{\cos^4 t}$
    56) $v = \frac{5}{\sin^3 2t}$
    57) $s = \frac{\sin t + \cos t}{2\sin 2t}$
    58) $z = \frac{\sin \alpha}{\alpha} + \frac{\alpha}{\sin \alpha}$
    59) $y = \frac{x \sin x}{1+\text{tg } x}$
    60) $y = \frac{x}{\sin x + \cos x}$
    61) $y = \cos x - \frac{1}{3}\cos^3 x$
    62) $y = \frac{1}{3}\sin^3 x - \frac{2}{5}\sin^5 x + \frac{1}{7}\sin^7 x$
    63) $y = \text{tg}^4 \sqrt{x}$
    64) $y = 3\text{ctg } x + \text{ctg}^3 x$
    65) $y = e^{ax}(a\sin x - \cos x)$
    66) $y = x^2 e^{2x} \sin x$
    67) $y = \cos^2 \frac{1}{\sqrt{x}}$
    68) $y = 2\sin^4 \frac{3}{\sqrt{x}}$
    69) $y = \frac{\sin^2 x}{\cos^7 x} - \frac{2}{5\cos^5 x}$
    70) $y = \frac{3\cos^2 x}{\sin^4 x}$
    71) $y = \sqrt{\sin x + \sqrt{x+2\sqrt{x}}}$
    72) $y = \sqrt{1+\text{tg}(x+\frac{1}{x})}$
    73) $z = \frac{3\text{tg } u - \text{tg}^3 u}{1-3\text{tg}^2 u}$
    74) $z = \text{tg } u - \text{ctg } u - 2u$
    75) $y = (4\sin x - 8\sin^3 x)\cos x$
    76) $y = \text{arctg } 3x$
    77) $y = 7\text{arctg } \frac{x}{2}$
    78) $x = \arcsin(1-t)$
    79) $x = \arccos \sqrt{1-t^2}$
    80) $x = \arcsin \sqrt{t^3}$
    81) $x = \arcsin \frac{1}{t}$
    82) $y = x\arcsin x + \sqrt{1-x^2}$, $0<x<1$
    83) $x = \arcsin(2t\sqrt{1-t^2})$
    84) $y = \text{arctg}(x-\sqrt{x^2+1})$
    85) $y = \text{arctg} \sqrt{x^2-1} - \frac{\ln x}{\sqrt{x^2-1}}$
    86) $y = x\text{arctg } x - \frac{1}{2}\ln(x^2+1)$
    87) $y = \frac{1}{6}x^5 \text{arctg } x - \frac{1}{24}x^4 + \frac{1}{12}x^2 - \frac{1}{12}\ln(1+x^2)$
    88) $y = \arcsin \frac{x}{\sqrt{1+x^2}}$
    89) $y = \arccos \sqrt{\frac{1-x^2}{1+x^2}}$
    90) $y = \text{arctg}\sqrt{\frac{1-x}{1+x}}$
    91) $y = \text{arctg}\frac{1+x}{1-x}$, $x \ne 1$
    92) $y = \text{arctg}\frac{x}{1+\sqrt{1+x^2}}$
    93) $y = \text{arctg}\frac{\sqrt{1+x^2}-1}{x}$
    94) $y = x^3 \text{arctg}^3 x$
    95) $z = \frac{\arcsin 4y}{1-4y}$
    96) $y = \frac{4}{\sqrt{3}}\text{arctg}\left[\frac{1}{\sqrt{3}}\left(2\text{tg}\frac{x}{2}+1\right)\right]-x$
    97) $y = \frac{1}{\sqrt{a^2-b^2}}\arcsin\frac{a \cos x+b}{a+b \cos x}$
    98) $y = e^{3x}$
    99) $y = 5e^{4x}$
    100) $y = e^{x^2}f(x)$
    101) $y = 3e^{-2x}g(x)$
    102) $y = e^{\sin x}$
    103) $y = 5e^{\cos x}$
    104) $y = e^{\cos^2 x}$
    105) $y = 3e^{2\sin^3 x}$
    106) $z = (v^3-3v^2+6v-6)e^v$
    107) $z = (10x^2-1)e^{3x}$
    108) $z = \frac{(2x-1)e^x}{2\sqrt{x}}$
    109) $y = (x+k\sqrt{1-x^2})e^{k \arcsin x}$
    110) $y = 5^x+2^x$
    111) $y = 3^x x^3$
    112) $y = 2^x \cdot 7^x - 1$
    113) $y = 5 \cdot 10^{3x}$
    114) $y = a^{2x}x^n$, $a>0$
    115) $y = \ln 3x$
    116) $y = 7 \cdot 5^{10x}$
    117) $z = \ln \frac{30}{x+3}$
    118) $y = 5\ln 10x$
    119) $s = \ln(t+\sqrt{t^2+1})$
    120) $z = 3\ln \frac{5}{x-2}$
    121) $s = \ln\sqrt{\frac{1+t}{1-t}}$
    122) $y = 2\ln \frac{3}{t+\sqrt{t^2-4}}$
    123) $y = \ln|\ln|x||$
    124) $y = \ln\frac{a+b \text{ tg } x}{a-b \text{ tg } x}$
    125) $y = \ln \text{tg}(\frac{\pi}{4}+\frac{x}{2})$, $0<x<\frac{\pi}{2}$
    126) $y = (\ln \cos \frac{x}{2})^2$
    127) $y = \ln \sqrt{\frac{1+\sin x}{1-\sin x}}$
    128) $y = 15\ln\text{tg}\frac{x}{2} + \frac{\cos x}{\sin^4 x}(8\cos^4 x - 25\cos^2 x + 15)$
    129) $y = \ln \sin x$
    130) $y = \ln \frac{1+\sqrt{x}}{1-\sqrt{x}}$, $0 \le x < 1$
    131) $y = \ln(1+\frac{a}{x})$
    132) $y = \ln(e^{mx}+e^{-mx})$
    133) $y = \log_x \ln x$. 
    134) $y = \log_x a$.
    135) $y = x^{5x}$, $x>0$
    136) $y = 10x^{-3x}$, $x>0$
    137) $y = x^{\sin x}$, $x>0$
    138) $y = 3x^{\cos x}$, $x>0$
    139) $y = (\frac{a}{x})^x$, $a>0, x>0$
    140) $y = x^{1/x}$, $x>0$
    141) $y = a^{\ln x}$, $a>0, x>0$
    142) $y = 5^{\sin 2x}$, $x>0$
    143) $y = x^{\ln x}$, $x>0$; wyjaśnić wynik.
    144) $y = (\sin x)^{\cos x}$, $0<x<\frac{\pi}{2}$
    145) $y = (\text{arctg } x)^x$, $x>0$
    146) $y = (\text{tg } x)^{\sin x}$, $0<x<\frac{\pi}{2}$
    147) $y = (\text{tg } x)^{1/\cos x}$, $0<x<\frac{\pi}{2}$
    148) $y = (\cos x)^{\text{ctg } x}$, $0<x<\frac{\pi}{2}$
    149) $y = e^{e^x}$
    150) $y = x^{e^x}$, $x>0$
    151) $y = x^{x^x}$, $x>0$
    152) $y = (1+\frac{1}{x})^x$
    153) $y = x^{\sqrt{\frac{1}{x}}}$